messageInvariantPrototypes/ringLeaderElection/automate_full/applicationProof.dfy
@@ -1,0 +1,182 @@
+include "messageInvariantsAutogen.dfy"
+
+module RingLeaderElectionProof {
+import opened Types
+import opened UtilitiesLibrary
+import opened DistributedSystem
+import opened Obligations
+import opened MessageInvariants
+
+  
+
+/***************************************************************************************
+*                                Application Invariants                                *
+***************************************************************************************/
+
+
+// Application bundle
+ghost predicate ApplicationInv(c: Constants, v: Variables)
+  requires v.WF(c)
+{
+  true
+}
+
+ghost predicate Inv(c: Constants, v: Variables)
+{
+  && v.WF(c)
+  && MessageInv(c, v)
+  && ApplicationInv(c, v)
+  && Safety(c, v)
+}
+
+ghost predicate Between(start: nat, node: nat, end: nat) 
+{
+  if start < end then
+    start < node < end else
+    node < end || start < node
+}
+
+function Distance(n: nat, start: nat, end: nat) : nat
+  requires 0 <= start < n
+  requires 0 <= end < n
+{
+  if start <= end then end - start 
+  else n - start + end
+}
+
+lemma InvImpliesSafety(c: Constants, v: Variables)
+  requires Inv(c, v)
+  ensures Safety(c, v)
+{}
+
+lemma InitImpliesInv(c: Constants, v: Variables)
+  requires Init(c, v)
+  ensures Inv(c, v)
+{
+  InitImpliesMessageInv(c, v);
+}
+
+lemma InvInductive(c: Constants, v: Variables, v': Variables)
+  requires Inv(c, v)
+  requires Next(c, v, v')
+  ensures Inv(c, v')
+{
+  MessageInvInductive(c, v, v');
+  MessageInvariantsImplyChordDominates(c, v');
+  ChordDominatesImpliesSafety(c, v');
+}
+
+/***************************************************************************************
+*                                        Proof                                         *
+***************************************************************************************/
+
+
+ghost predicate ChordDominates(c: Constants, v: Variables) 
+  requires v.WF(c)
+{
+  forall i:int, src:nat, dst:nat, mid:nat | 
+      && v.ValidHistoryIdx(i)
+      && c.ValidIdx(src)
+      && c.ValidIdx(dst)
+      && c.ValidIdx(mid)
+      && v.History(i).hosts[dst].highestHeard == c.hosts[src].hostId
+      && Between(src, mid, dst)
+    :: 
+      c.hosts[mid].hostId < c.hosts[src].hostId
+}
+
+lemma ChordDominatesImpliesSafety(c: Constants, v: Variables)
+  requires v.WF(c)
+  requires ChordDominates(c, v)
+  ensures Safety(c, v)
+{}
+
+lemma MessageInvariantsImplyChordDominates(c: Constants, v: Variables)
+  requires v.WF(c)
+  requires MessageInv(c, v)
+  ensures ChordDominates(c, v)
+{
+  forall i:int, src:nat, dst:nat, mid:nat | 
+    && v.ValidHistoryIdx(i)
+    && c.ValidIdx(src)
+    && c.ValidIdx(dst)
+    && c.ValidIdx(mid)
+    && v.History(i).hosts[dst].highestHeard == c.hosts[src].hostId
+    && Between(src, mid, dst)
+  ensures
+    c.hosts[mid].hostId < c.hosts[src].hostId
+  {
+    reveal_ReceiveMsgValidity();
+    var hh := v.History(i).hosts[dst].highestHeard;
+    assert Host.ReceiveMsgTrigger(c.hosts[dst], v.History(i).hosts[dst], hh); // trigger
+    var pred := Predecessor(|c.hosts|, dst);
+    assert Between(src, pred, dst);
+    if pred != mid {
+      MidMustHaveSentSrcHostId(c, v, src, mid, dst, i);
+    }
+  }
+}
+
+lemma MidMustHaveSentSrcHostId(c: Constants, v: Variables, src: nat, mid: nat, dst: nat, i:nat) 
+  requires v.WF(c)
+  requires MessageInv(c, v)
+  requires c.ValidIdx(src)
+  requires c.ValidIdx(dst)
+  requires c.ValidIdx(mid)
+  requires v.ValidHistoryIdx(i)
+  requires v.History(i).hosts[dst].highestHeard == c.hosts[src].hostId
+  requires Between(src, mid, dst)
+  ensures Msg(c.hosts[src].hostId, mid) in v.network.sentMsgs 
+  decreases Distance(|c.hosts|, mid, dst)
+{
+  LemmaSentNotMyIdImpliesReceivedId(c, v);
+  var n := |c.hosts|;
+  if mid == Predecessor(n, dst) {
+    // by receiveValidity
+    reveal_ReceiveMsgValidity();
+    var hh := v.History(i).hosts[dst].highestHeard;
+    assert Host.ReceiveMsgTrigger(c.hosts[dst], v.History(i).hosts[dst], hh);
+    assert Msg(c.hosts[src].hostId, mid) in v.network.sentMsgs;
+  } else {
+    reveal_ReceiveMsgValidity();
+    var succ := Successor(n, mid);
+    SuccessorDecreasesDistance(n, mid, dst);
+    MidMustHaveSentSrcHostId(c, v, src, succ, dst, i);
+  }
+}
+
+lemma SuccessorDecreasesDistance(n:nat, start:nat, end:nat) 
+  requires 0 <= start < n
+  requires 0 <= end < n
+  requires start != end
+  ensures Distance(n, start, end) > Distance(n, Successor(n, start), end)
+{}
+
+ghost predicate SentNotMyIdImpliesReceivedId(c: Constants, v: Variables) 
+  requires v.WF(c)
+  requires MessageInv(c, v)
+{
+  var n := |c.hosts|;
+  forall msg | msg in v.network.sentMsgs && msg.val != c.hosts[msg.src].hostId 
+  :: Msg(msg.val, Predecessor(n, msg.src)) in v.network.sentMsgs
+}
+
+lemma LemmaSentNotMyIdImpliesReceivedId(c: Constants, v: Variables)
+  requires v.WF(c)
+  requires MessageInv(c, v)
+  ensures SentNotMyIdImpliesReceivedId(c, v)
+{
+  reveal_ReceiveMsgValidity();
+  var n := |c.hosts|;
+  forall msg | msg in v.network.sentMsgs && msg.val != c.hosts[msg.src].hostId 
+  ensures Msg(msg.val, Predecessor(n, msg.src)) in v.network.sentMsgs
+  {
+    var i :| 
+      && v.ValidHistoryIdxStrict(i)
+      && Host.SendMsg(c.hosts[msg.Src()], v.History(i).hosts[msg.Src()], v.History(i+1).hosts[msg.Src()], msg);
+    assert Host.ReceiveMsgTrigger(c.hosts[msg.src], v.History(i).hosts[msg.src], msg.val);  // trigger
+  }
+}
+
+}  // end module RingLeaderElectionProof
+
